wip: add some fetch Hoare triples

CHERI_Fetch_Properties.thy
@@ -1,5 +1,5 @@
 theory CHERI_Fetch_Properties
-  imports CHERI_Mem_Properties
+  imports CHERI_Mem_Properties "Sail.Hoare"
 begin
 
 context Morello_Fetch_Automaton
@@ -36,6 +36,357 @@ lemma traces_enabled_FetchInstr[traces_enabledI]:
   shows "traces_enabled (FetchInstr pc) s"
   unfolding FetchInstr_def CheckPCCCapability_def bind_assoc
   by (traces_enabledI assms: assms elim: CheckCapability_load_enabled intro: derivable_or_invokedI1)
+
+end
+
+lemma Run_Read_mem_iff:
+  "Run (Read_mem rk addr sz k) t a \<longleftrightarrow> (\<exists>t' data. t = E_read_mem rk addr sz data # t' \<and> Run (k data) t' a)"
+  by (auto elim: Traces_cases)
+
+lemma Value_returnS_iff[simp]:
+  "(Value x, s') \<in> returnS a s \<longleftrightarrow> x = a \<and> s' = s"
+  by (auto simp: returnS_def)
+
+lemma Value_readS_iff[simp]:
+  "(Value a, s') \<in> readS f s \<longleftrightarrow> a = f s \<and> s' = s"
+  by (auto simp: readS_def)
+
+lemma Value_updateS_iff[simp]:
+  "(Value u, s') \<in> updateS f s \<longleftrightarrow> s' = f s"
+  by (auto simp: updateS_def)
+
+lemma Value_throwS_False[simp]:
+  "(Value a, s') \<in> throwS ex s \<longleftrightarrow> False"
+  by (auto simp: throwS_def)
+
+lemma Value_failS_False[simp]:
+  "(Value a, s') \<in> failS msg s \<longleftrightarrow> False"
+  by (auto simp: failS_def)
+
+lemma Value_maybe_failS_iff[simp]:
+  "(Value a, s') \<in> maybe_failS msg x s \<longleftrightarrow> x = Some a \<and> s' = s"
+  by (auto simp: maybe_failS_def split: option.splits)
+
+lemma Value_read_memt_bytesS_iff[simp]:
+  "(Value data, s') \<in> read_memt_bytesS rk a sz s \<longleftrightarrow> get_mem_bytes a sz s = Some data \<and> s' = s"
+  by (auto simp: read_memt_bytesS_def elim!: Value_bindS_elim intro: bindS_intros)
+
+lemma Value_read_mem_bytesS_iff[simp]:
+  "(Value data, s') \<in> read_mem_bytesS rk a sz s \<longleftrightarrow> (\<exists>tag. get_mem_bytes a sz s = Some (data, tag) \<and> s' = s)"
+  by (auto simp: read_mem_bytesS_def elim!: Value_bindS_elim intro: bindS_intros)
+
+lemma Value_write_memt_bytesS_iff[simp]:
+  "(Value b, s') \<in> write_memt_bytesS wk a sz data tag s \<longleftrightarrow> s' = put_mem_bytes a sz data tag s \<and> b"
+  by (auto simp: write_memt_bytesS_def elim!: Value_bindS_elim intro: bindS_intros)
+
+lemma Value_write_mem_bytesS_iff[simp]:
+  "(Value b, s') \<in> write_mem_bytesS wk a sz data s \<longleftrightarrow> s' = put_mem_bytes a sz data B0 s \<and> b"
+  by (auto simp: write_mem_bytesS_def elim!: Value_bindS_elim intro: bindS_intros)
+
+lemma Value_read_regvalS_iff[simp]:
+  "(Value a, s') \<in> read_regvalS ra r s \<longleftrightarrow> fst ra r (regstate s) = Some a \<and> s' = s"
+  by (cases ra; auto elim!: Value_bindS_elim intro: bindS_intros split: option.splits)
+
+lemma Value_write_regvalS_iff[simp]:
+  "(Value u, s') \<in> write_regvalS ra r a s \<longleftrightarrow> (\<exists>rs'. snd ra r a (regstate s) = Some rs' \<and> s' = s\<lparr>regstate := rs'\<rparr>)"
+  by (cases ra; auto elim!: Value_bindS_elim intro: bindS_intros split: option.splits)
+
+lemma Value_chooseS_iff[simp]:
+  "(Value x, s') \<in> chooseS xs s \<longleftrightarrow> x \<in> xs \<and> s' = s"
+  by (auto simp: chooseS_def)
+
+lemma Value_choose_boolS_iff[simp]:
+  "(Value x, s') \<in> choose_boolS msg s \<longleftrightarrow> s' = s"
+  by (auto simp: choose_boolS_def)
+
+declare excl_resultS_def[simp]
+
+lemma Value_liftState_Run_runTraceS:
+  assumes "(Value a, s') \<in> liftState r m s"
+  obtains t where "Run m t a" and "runTraceS r t s = Some s'"
+(*proof -
+  from assms obtain t where "Run m t a"
+    by (elim Value_liftState_Run)
+  with assms that show thesis
+    apply (induction r t s rule: runTraceS.induct)
+    apply auto*)
+proof (use assms in \<open>induction r m arbitrary: s s' rule: liftState.induct\<close>)
+  case (1 ra a)
+  then show ?case by (simp)
+next
+  case (2 ra rk a sz k)
+  (*then show ?case
+    apply (auto elim!: Value_bindS_elim simp add: returnS_def maybe_failS_def failS_def readS_def read_mem_bytesS_def read_memt_bytesS_def bind_eq_Some_conv split: option.splits)
+    apply (auto elim!: Value_bindS_elim intro: Traces_ConsI) *)
+  then show ?case
+    by (force elim!: Value_bindS_elim intro: Traces_ConsI)
+    (*thm "2.IH"[rotated -1]
+    apply (erule "2.IH"[rotated -1])
+     apply blast
+    apply (rule "2.prems")
+     apply (rule Traces_ConsI)
+     apply assumption
+    apply (auto elim!: Value_bindS_elim)
+    thm runTraceS.induct emitEventS.elims
+    sorry*)
+next
+  case (3 ra rk a sz k)
+  then show ?case
+    by (force elim!: Value_bindS_elim intro: Traces_ConsI)
+next
+  case (4 ra wk a sz v k)
+  then show ?case
+    by (fastforce elim!: Value_bindS_elim intro: Traces_ConsI)
+next
+  case (5 ra wk a sz v t k)
+  then show ?case by (fastforce elim!: Value_bindS_elim intro: Traces_ConsI)
+next
+  case (6 ra r k)
+  then show ?case by (force elim!: Value_bindS_elim intro: Traces_ConsI)
+next
+  case (7 ra k)
+  then show ?case by (force elim!: Value_bindS_elim intro: Traces_ConsI)
+next
+case (8 ra uu k)
+  then show ?case by (force elim!: Value_bindS_elim intro: Traces_ConsI)
+next
+  case (9 ra r v k)
+  then show ?case by (force elim!: Value_bindS_elim intro: Traces_ConsI)
+next
+  case (10 ra uv uw ux k)
+  then show ?case by (force elim!: Value_bindS_elim intro: Traces_ConsI)
+next
+  case (11 ra k)
+  then show ?case by (force elim!: Value_bindS_elim intro: Traces_ConsI)
+next
+  case (12 ra uy k)
+  then show ?case by (force elim!: Value_bindS_elim intro: Traces_ConsI)
+next
+  case (13 ra uz k)
+  then show ?case by (force elim!: Value_bindS_elim intro: Traces_ConsI)
+next
+  case (14 ra descr)
+  then show ?case by (force elim!: Value_bindS_elim intro: Traces_ConsI)
+next
+  case (15 ra e)
+  then show ?case by (force elim!: Value_bindS_elim intro: Traces_ConsI)
+qed
+
+lemma PrePostE_exp_fails:
+  assumes "exp_fails m"
+  shows "\<lbrace>P\<rbrace> \<lbrakk>m\<rbrakk>\<^sub>S \<lbrace>Q \<bar> \<lambda>_ _. True\<rbrace>"
+  using assms
+  by (intro PrePostE_I) (auto elim: Value_liftState_Run)
+
+lemma PrePostE_any_no_ex:
+  "PrePostE (\<lambda>s. \<forall>a s'. (Value a, s') \<in> m s \<longrightarrow> Q a s') m Q (\<lambda>_ _. True)"
+  by (rule PrePostE_I)  auto
+
+declare PrePostE_True_post[PrePostE_atomI del]
+
+fun no_reg_writes_trace where
+  "no_reg_writes_trace (E_write_reg _ _ # _) = False"
+| "no_reg_writes_trace (_ # t) = no_reg_writes_trace t"
+| "no_reg_writes_trace [] = True"
+
+lemma no_reg_writes_trace_iff:
+  "no_reg_writes_trace t \<longleftrightarrow> (\<forall>r v. E_write_reg r v \<notin> set t)"
+  by (induction t rule: no_reg_writes_trace.induct; auto)
+
+lemma Run_no_reg_writes_trace:
+  assumes "Run m t a" and "runs_no_reg_writes_to UNIV m"
+  shows "no_reg_writes_trace t"
+  using assms
+  by (auto simp: runs_no_reg_writes_to_def no_reg_writes_trace_iff)
+
+lemma regstate_put_mem_bytes[simp]:
+  "regstate (put_mem_bytes addr sz v tag s) = regstate s"
+  by (auto simp: put_mem_bytes_def Let_def)
+
+lemma no_reg_writes_trace_regstate_eq:
+  assumes "runTraceS ra t s = Some s'" and "no_reg_writes_trace t"
+  shows "regstate s' = regstate s"
+  using assms
+  by (induction t arbitrary: s rule: no_reg_writes_trace.induct) (auto split: bind_splits if_splits)
+
+lemma PrePostE_no_reg_writes:
+  assumes m: "runs_no_reg_writes_to UNIV m"
+    and pp: "\<And>s0. \<lbrace>\<lambda>s. s0 = s \<and> P s\<rbrace> liftState ra m \<lbrace>\<lambda>a s. regstate s = regstate s0 \<longrightarrow> Q a s \<bar> E\<rbrace>"
+  shows "\<lbrace>P\<rbrace> liftState ra m \<lbrace>Q \<bar> E\<rbrace>"
+proof (rule PrePostE_I)
+  fix s a s'
+  assume "P s" and s': "(Value a, s') \<in> liftState ra m s"
+  then obtain t where "Run m t a" and t: "runTraceS ra t s = Some s'"
+    by (elim Value_liftState_Run_runTraceS)
+  then show "Q a s'"
+    using \<open>P s\<close> m pp[of s] s' no_reg_writes_trace_regstate_eq[OF t]
+    by (elim PrePostE_elim[where s = s and s' = s' and r = "Value a"])
+       (auto simp: intro: Run_no_reg_writes_trace)
+next
+  fix s e s'
+  assume "P s" and "(Ex e, s') \<in> liftState ra m s"
+  then show "E e s'"
+    using pp[of s]
+    by (auto elim: PrePostE_elim)
+qed
+
+fun no_mem_writes_trace where
+  "no_mem_writes_trace (E_write_memt _ _ _ _ _ _ # _) = False"
+| "no_mem_writes_trace (E_write_mem _ _ _ _ _ # _) = False"
+| "no_mem_writes_trace (_ # t) = no_mem_writes_trace t"
+| "no_mem_writes_trace [] = True"
+
+lemma no_mem_writes_trace_iff:
+  "no_mem_writes_trace t \<longleftrightarrow>
+     (\<forall>wk addr sz data tag s.
+        E_write_memt wk addr sz data tag s \<notin> set t \<and>
+        E_write_mem wk addr sz data s \<notin> set t)"
+  by (induction t rule: no_mem_writes_trace.induct; fastforce)
+
+definition "runs_no_mem_writes m \<equiv> (\<forall>t a. Run m t a \<longrightarrow> no_mem_writes_trace t)"
+
+lemma no_mem_writes_trace_append[simp]:
+  "no_mem_writes_trace (t1 @ t2) \<longleftrightarrow> no_mem_writes_trace t1 \<and> no_mem_writes_trace t2"
+  by (induction t1 rule: no_mem_writes_trace.induct) auto
+
+lemma runs_no_mem_writes_bind:
+  assumes "runs_no_mem_writes m" and "\<And>t a. Run m t a \<Longrightarrow> runs_no_mem_writes (f a)"
+  shows "runs_no_mem_writes (bind m f)"
+  using assms
+  by (fastforce simp: runs_no_mem_writes_def elim!: Run_bindE)
+
+lemmas runs_no_mem_writes_if_split = if_split[of runs_no_mem_writes, THEN iffD2]
+
+lemma no_mem_writes_trace_memstate_eq:
+  assumes "runTraceS ra t s = Some s'" and "no_mem_writes_trace t"
+  shows "memstate s' = memstate s" and "tagstate s' = tagstate s"
+  using assms
+  by (induction t arbitrary: s rule: no_mem_writes_trace.induct) (auto split: bind_splits if_splits)
+
+lemma no_reg_mem_writes_state_eq:
+  assumes "runTraceS ra t s = Some s'"
+    and "no_reg_writes_trace t" and "no_mem_writes_trace t"
+  shows "s' = s"
+  using assms
+  by (intro sequential_state.equality)
+     (auto simp: no_reg_writes_trace_regstate_eq no_mem_writes_trace_memstate_eq)
+
+context Cap_Axiom_Automaton
+begin
+
+lemma non_mem_no_mem_writes_trace:
+  assumes "non_mem_trace t"
+  shows "no_mem_writes_trace t"
+  using assms
+  by (induction t rule: no_mem_writes_trace.induct) auto
+
+lemma non_mem_exp_runs_no_mem_writes:
+  assumes "non_mem_exp m"
+  shows "runs_no_mem_writes m"
+  using assms
+  by (auto simp: non_mem_exp_def runs_no_mem_writes_def intro: non_mem_no_mem_writes_trace)
+
+lemma PrePostE_no_writes:
+  assumes m: "runs_no_reg_writes_to UNIV m" "runs_no_mem_writes m"
+    and pp: "\<And>s0. \<lbrace>\<lambda>s. s0 = s \<and> P s\<rbrace> liftState ra m \<lbrace>\<lambda>a s. s = s0 \<longrightarrow> Q a s \<bar> E\<rbrace>"
+  shows "\<lbrace>P\<rbrace> liftState ra m \<lbrace>Q \<bar> E\<rbrace>"
+proof (rule PrePostE_I)
+  fix s a s'
+  assume "P s" and s': "(Value a, s') \<in> liftState ra m s"
+  then obtain t where "Run m t a" and t: "runTraceS ra t s = Some s'"
+    by (elim Value_liftState_Run_runTraceS)
+  then show "Q a s'"
+    using \<open>P s\<close> m pp[of s] s' no_reg_mem_writes_state_eq[OF t]
+    by (elim PrePostE_elim[where s = s and s' = s' and r = "Value a"])
+       (auto simp: runs_no_mem_writes_def intro: Run_no_reg_writes_trace)
+next
+  fix s e s'
+  assume "P s" and "(Ex e, s') \<in> liftState ra m s"
+  then show "E e s'"
+    using pp[of s]
+    by (auto elim: PrePostE_elim)
+qed
+
+lemma PrePostE_no_writes_any_runs:
+  assumes m: "runs_no_reg_writes_to UNIV m" "runs_no_mem_writes m"
+  shows "\<lbrace>P\<rbrace> liftState ra m \<lbrace>\<lambda>_. P \<bar> \<lambda>_ _. True\<rbrace>"
+  by (rule PrePostE_no_writes[OF assms]) (auto intro: PrePostE_I)
+
+end
+
+context Morello_Axiom_Automaton
+begin
+
+lemma PrePostE_CheckCapability_tagged_unsealed:
+  shows "\<lbrace>\<lambda>s. CapIsTagSet c \<and> \<not>CapIsSealed c \<longrightarrow> Q addr s\<rbrace>
+           \<lbrakk>CheckCapability c addr sz perms acctype\<rbrakk>\<^sub>S
+         \<lbrace>Q \<bar> \<lambda>_ _. True\<rbrace>"
+  unfolding CheckCapability_def bind_assoc
+  apply (rule PrePostE_no_writes)
+    apply (no_reg_writes_toI)
+   apply (rule non_mem_exp_runs_no_mem_writes)
+  apply (non_mem_expI)
+  apply (rule PrePostE_I)
+   apply (auto elim!: Value_liftState_Run Run_bindE split: if_splits)
+  done
+
+abbreviation "getPCC s \<equiv> bitvector_129_dec_reg (regstate s) ''PCC''"
+
+lemma runs_no_reg_writes_to_AArch64_CheckIllegalState[runs_no_reg_writes_toI, simp]:
+  "runs_no_reg_writes_to Rs (AArch64_CheckIllegalState u)"
+  by (unfold AArch64_CheckIllegalState_def, no_reg_writes_toI)
+
+lemma runs_no_mem_writes_Mem_read:
+  "runs_no_mem_writes (Mem_read desc sz accdesc)"
+  unfolding Mem_read_def read_mem_def read_mem_bytes_def maybe_fail_def
+  by (auto simp: runs_no_mem_writes_def Run_Read_mem_iff elim!: Run_bindE split: option.splits)
+
+lemma runs_no_mem_writes_AArch64_MemSingle_read:
+  "runs_no_mem_writes (AArch64_MemSingle_read addr sz acctype wasaligned)"
+  unfolding AArch64_MemSingle_read_def Let_def
+  by (intro runs_no_mem_writes_bind runs_no_mem_writes_if_split runs_no_mem_writes_Mem_read
+            non_mem_exp_runs_no_mem_writes conjI impI;
+      non_mem_expI)
+
+lemma
+  shows "\<lbrace>\<lambda>_. True\<rbrace> \<lbrakk>FetchInstr pc\<rbrakk>\<^sub>S \<lbrace>\<lambda>_ s. CapIsTagSet (getPCC s) \<and> \<not>CapIsSealed (getPCC s) \<bar> \<lambda>_ _. True\<rbrace>"
+  unfolding FetchInstr_def CheckPCCCapability_def bind_assoc
+  unfolding liftState_simp comp_def Let_def
+  apply (rule PrePostE_strengthen_pre)
+  apply (rule PrePostE_compositeI PrePostE_atomI)+
+             apply (rule PrePostE_no_writes_any_runs)
+              apply (no_reg_writes_toI)
+              apply (rule non_mem_exp_runs_no_mem_writes)
+              apply (non_mem_expI)
+             apply (rule PrePostE_no_writes_any_runs)
+               apply (no_reg_writes_toI)
+             apply (rule runs_no_mem_writes_AArch64_MemSingle_read)
+              apply (rule PrePostE_CheckCapability_tagged_unsealed)
+             apply (rule PrePostE_atomI)
+            apply (rule PrePostE_atomI)
+           apply (rule PrePostE_no_writes_any_runs)
+            apply (no_reg_writes_toI)
+           apply (rule non_mem_exp_runs_no_mem_writes)
+           apply (non_mem_expI)
+          apply (rule PrePostE_no_writes_any_runs)
+           apply (no_reg_writes_toI)
+          apply (rule non_mem_exp_runs_no_mem_writes)
+          apply (non_mem_expI)
+         apply (rule PrePostE_compositeI PrePostE_atomI)+
+       apply (rule PrePostE_no_writes_any_runs)
+        apply (no_reg_writes_toI)
+       apply (rule non_mem_exp_runs_no_mem_writes)
+       apply (non_mem_expI)
+       apply (rule PrePostE_no_writes_any_runs)
+       apply (no_reg_writes_toI)
+      apply (rule non_mem_exp_runs_no_mem_writes)
+      apply (non_mem_expI)
+      apply (rule PrePostE_no_writes_any_runs)
+      apply (no_reg_writes_toI)
+      apply (rule non_mem_exp_runs_no_mem_writes)
+      apply (non_mem_expI)
+     apply (simp add: PCC_ref_def)
+  done
 
 end
 
